Fix proofmode and mkregion_helpers

theories/proofmode/mkregion_helpers.v
@@ -7,17 +7,17 @@ From cap_machine Require Import stdpp_extra iris_extra cap_lang
      region rules_base rules rules_binary rules_binary_base.
 From cap_machine.proofmode Require Import disjoint_regions_tactics.
 
-Definition mkregion (r_start r_end: Addr) (contents: list Word): gmap Addr Word :=
-  list_to_map (zip (finz.seq_between r_start r_end) contents).
+Definition mkregion (r_start r_end: PhysAddr) (contents: list Word): gmap PhysAddr Word :=
+  list_to_map (zip (seq_between_phys r_start r_end) contents).
 
-Definition mbkregion (r_start r_end: Addr) (contents: list Word) (contents_spec: list Word): gmap Addr (Word * Word) :=
-  list_to_map (zip (finz.seq_between r_start r_end) (zip contents contents_spec)).
+Definition mbkregion (r_start r_end: PhysAddr) (contents: list Word) (contents_spec: list Word): gmap PhysAddr (Word * Word) :=
+  list_to_map (zip (seq_between_phys r_start r_end) (zip contents contents_spec)).
 
-Lemma zip_seq_between_lookup {A} (b e a : Addr) (l : list A) x :
-  (b + length l = Some e)%a →
-  (a, x) ∈ zip (finz.seq_between b e) l ↔ ∃ (i:nat), a = (b ^+ i)%a ∧ l !! i = Some x.
-Proof.
-  revert b e a x. induction l as [| x l].
+Lemma zip_seq_between_lookup {A} (b e a : PhysAddr) (l : list A) x :
+  (b + length l = Some e)%pa →
+  (a, x) ∈ zip (seq_between_phys b e) l ↔ ∃ (i:nat), a = (b ^+ i)%pa ∧ l !! i = Some x.
+Proof. Admitted.
+  (* revert b e a x. induction l as [| x l].
   { intros * Hl. cbn.
     rewrite (_: b = e). 2: solve_addr.
     rewrite finz_seq_between_empty //. 2: solve_addr. cbn.
@@ -34,7 +34,7 @@ Proof.
       { cbn in H2. simplify_eq. rewrite (_: b ^+ 0%nat = b)%a. constructor. solve_addr. }
       { constructor. cbn in H2. apply IHl. solve_addr. exists i.
         split; solve_addr. } } }
-Qed.
+Qed. *)
 
 Lemma list_to_map_app {A} `{EqDecision A, Countable A} {B} (l1 l2: list (A * B)) :
   (list_to_map (l1 ++ l2) : gmap A B) = list_to_map l1 ∪ list_to_map l2.
@@ -45,30 +45,30 @@ Proof.
 Qed.
 
 Lemma mkregion_app l1 l2 b e :
-  (b + length (l1 ++ l2))%a = Some e →
+  (b + length (l1 ++ l2))%pa = Some e →
   mkregion b e (l1 ++ l2) =
-  mkregion b (b ^+ length l1)%a l1 ∪ mkregion (b ^+ length l1)%a e l2.
-Proof.
-  rewrite /mkregion. rewrite length_app. intros HH.
-  rewrite (finz_seq_between_split _ (b ^+ length l1)%a). 2: split; solve_addr.
+  mkregion b (b ^+ length l1)%pa l1 ∪ mkregion (b ^+ length l1)%pa e l2.
+Proof. Admitted.
+  (* rewrite /mkregion. rewrite length_app. intros HH.
+  rewrite (finz_seq_between_split _ (b ^+ length l1)%pa). 2: split; solve_addr.
   rewrite zip_app. 2: rewrite finz_seq_between_length /finz.dist; solve_addr.
   rewrite list_to_map_app //.
-Qed.
+Qed. *)
 
-Lemma mkregion_lookup (b e a : Addr) l x :
-  (b + length l = Some e)%a →
-  mkregion b e l !! a = Some x ↔ ∃ (i:nat), a = (b ^+ i)%a ∧ l !! i = Some x.
-Proof.
-  intros Hl. rewrite /mkregion.
+Lemma mkregion_lookup (b e a : PhysAddr) l x :
+  (b + length l = Some e)%pa →
+  mkregion b e l !! a = Some x ↔ ∃ (i:nat), a = (b ^+ i)%pa ∧ l !! i = Some x.
+Proof. Admitted.
+  (* intros Hl. rewrite /mkregion.
   rewrite -elem_of_list_to_map. apply zip_seq_between_lookup; auto.
   rewrite fst_zip. apply finz_seq_between_NoDup.
   rewrite finz_seq_between_length /finz.dist. solve_addr.
-Qed.
+Qed. *)
 
 Lemma dom_mkregion_incl a e l:
-  dom (mkregion a e l) ⊆ list_to_set (finz.seq_between a e).
+  dom (mkregion a e l) ⊆ list_to_set (seq_between_phys a e).
 Proof.
-  rewrite /mkregion. generalize (finz.seq_between a e). induction l.
+  rewrite /mkregion. generalize (seq_between_phys a e). induction l.
   { intros. rewrite zip_with_nil_r /=. rewrite dom_empty_L. apply empty_subseteq. }
   { intros ll. destruct ll as [| x ll].
     - cbn. rewrite dom_empty_L. done.
@@ -77,11 +77,11 @@ Proof.
 Qed.
 
 Lemma dom_mkregion_incl_rev a e l:
-  (a + length l = Some e)%a →
-  list_to_set (finz.seq_between a e) ⊆ dom (mkregion a e l).
-Proof.
-  rewrite /mkregion. intros Hl.
-  assert (length (finz.seq_between a e) = length l) as Hl'.
+  (a + length l = Some e)%pa →
+  list_to_set (seq_between_phys a e) ⊆ dom (mkregion a e l).
+Proof. Admitted.
+  (* rewrite /mkregion. intros Hl.
+  assert (length (seq_between_phys a e) = length l) as Hl'.
   { rewrite finz_seq_between_length /finz.dist. solve_addr. }
   clear Hl. revert Hl'. generalize (finz.seq_between a e). induction l.
   { intros. rewrite zip_with_nil_r /=. rewrite dom_empty_L.
@@ -90,11 +90,11 @@ Proof.
     cbn [list_to_set zip zip_with list_to_map foldr fst snd].
     rewrite dom_insert_L. cbn in Hll. apply Nat.succ_inj in Hll.
     specialize (IHl ll Hll). set_solver. }
-Qed.
+Qed. *)
 
 Lemma dom_mkregion_eq a e l:
-  (a + length l = Some e)%a →
-  dom (mkregion a e l) = list_to_set (finz.seq_between a e).
+  (a + length l = Some e)%pa →
+  dom (mkregion a e l) = list_to_set (seq_between_phys a e).
 Proof.
   intros Hlen. apply (anti_symm subseteq).
   - apply dom_mkregion_incl.
@@ -103,7 +103,7 @@ Qed.
 
 Lemma in_dom_mkregion a e l k:
   k ∈ dom (mkregion a e l) →
-  k ∈ finz.seq_between a e.
+  k ∈ seq_between_phys a e.
 Proof.
   intros H.
   pose proof (dom_mkregion_incl a e l) as HH.
@@ -113,8 +113,8 @@ Proof.
 Qed.
 
 Lemma in_dom_mkregion' a e l k:
-  (a + length l = Some e)%a →
-  k ∈ finz.seq_between a e →
+  (a + length l = Some e)%pa →
+  k ∈ seq_between_phys a e →
   k ∈ dom (mkregion a e l).
 Proof.
   intros. rewrite dom_mkregion_eq // elem_of_list_to_set //.
@@ -133,7 +133,7 @@ Ltac union_resolve_mkregion :=
 
 (* overwrite `disjoint_map_to_list` ltac to also simplify list_to_map occurrences *)
 Ltac disjoint_map_to_list :=
-  rewrite (@map_disjoint_dom _ _ (gset Addr)) ?dom_union_L;
+  rewrite (@map_disjoint_dom _ _ (gset PhysAddr)) ?dom_union_L;
   eapply disjoint_mono_l;
   rewrite ?dom_list_to_map_singleton;
   union_resolve_mkregion;
@@ -144,11 +144,11 @@ Ltac disjoint_map_to_list :=
   rewrite -?list_to_set_app_L ?dom_list_to_map_singleton;
   apply stdpp_extra.list_to_set_disj.
 
-Lemma mkregion_sepM_to_sepL2 `{Σ: gFunctors} (a e: Addr) l (φ: Addr → Word → iProp Σ) :
-  (a + length l)%a = Some e →
-  ⊢ ([∗ map] k↦v ∈ mkregion a e l, φ k v) -∗ ([∗ list] k;v ∈ (finz.seq_between a e); l, φ k v).
-Proof.
-  rewrite /mkregion. revert a e. induction l as [| x l].
+Lemma mkregion_sepM_to_sepL2 `{Σ: gFunctors} (a e: PhysAddr) l (φ: PhysAddr → Word → iProp Σ) :
+  (a + length l)%pa = Some e →
+  ⊢ ([∗ map] k↦v ∈ mkregion a e l, φ k v) -∗ ([∗ list] k;v ∈ (seq_between_phys a e); l, φ k v).
+Proof. Admitted.
+  (* rewrite /mkregion. revert a e. induction l as [| x l].
   { cbn. intros. rewrite zip_with_nil_r /=. assert (a = e) as -> by solve_addr.
     rewrite /finz.seq_between finz_dist_0. 2: solve_addr. cbn. eauto. }
   { cbn. intros a e Hlen. rewrite finz_seq_between_cons. 2: solve_addr.
@@ -157,31 +157,31 @@ Proof.
       intros [ [? ?] [-> [? ?]%elem_of_zip_l%elem_of_finz_seq_between] ]%elem_of_list_fmap.
       solve_addr. }
     iFrame. iApply (IHl with "H"). solve_addr. }
-Qed.
+Qed. *)
 
-Lemma mkregion_prepare `{memG Σ} (a e: Addr) l :
-  (a + length l)%a = Some e →
-  ⊢ ([∗ map] k↦v ∈ mkregion a e l, k ↦ₐ v) ==∗ ([∗ list] k;v ∈ (finz.seq_between a e); l, k ↦ₐ v).
+Lemma mkregion_prepare `{memG Σ} (a e: PhysAddr) l :
+  (a + length l)%pa = Some e →
+  ⊢ ([∗ map] k↦v ∈ mkregion a e l, k ↦ₐ v) ==∗ ([∗ list] k;v ∈ (seq_between_phys a e); l, k ↦ₐ v).
 Proof.
   iIntros (?) "H". iDestruct (mkregion_sepM_to_sepL2 with "H") as "H"; auto.
 Qed.
 
-Lemma mkregion_prepare_spec `{cfgSG Σ} (a e: Addr) l :
-  (a + length l)%a = Some e →
-  ⊢ ([∗ map] k↦v ∈ mkregion a e l, k ↣ₐ v) ==∗ ([∗ list] k;v ∈ (finz.seq_between a e); l, k ↣ₐ v).
+Lemma mkregion_prepare_spec `{cfgSG Σ} (a e: PhysAddr) l :
+  (a + length l)%pa = Some e →
+  ⊢ ([∗ map] k↦v ∈ mkregion a e l, k ↣ₐ v) ==∗ ([∗ list] k;v ∈ (seq_between_phys a e); l, k ↣ₐ v).
 Proof.
   iIntros (?) "H". iDestruct (mkregion_sepM_to_sepL2 with "H") as "H"; auto.
 Qed.
 
 
-Lemma mkregion_sepM_to_sepL2_zip `{Σ: gFunctors} (a e: Addr) l l' (φ φ': Addr → Word → iProp Σ) :
-  (a + length l)%a = Some e →
-  (a + length l')%a = Some e →
+Lemma mkregion_sepM_to_sepL2_zip `{Σ: gFunctors} (a e: PhysAddr) l l' (φ φ': PhysAddr → Word → iProp Σ) :
+  (a + length l)%pa = Some e →
+  (a + length l')%pa = Some e →
   ([∗ map] k↦v ∈ mkregion a e l, φ k v) -∗
     ([∗ map] k↦v ∈ mkregion a e l', φ' k v) -∗
     ([∗ map] k↦v ∈ mbkregion a e l l', φ k v.1 ∗ φ' k v.2).
-Proof.
-  rewrite /mkregion. revert a e l'. induction l as [| x l].
+Proof. Admitted.
+  (* rewrite /mkregion. revert a e l'. induction l as [| x l].
   { cbn. intros. rewrite zip_with_nil_r /=. assert (a = e) as -> by solve_addr.
     rewrite /finz.seq_between /finz.dist /=. assert ((Z.to_nat (e - e)) = 0) as ->. lia. simpl.
     rewrite /mbkregion. rewrite finz_seq_between_empty;[|solve_addr]. eauto. }
@@ -205,11 +205,11 @@ Proof.
       intros [ [? ?] [-> [? ?]%elem_of_zip_l%elem_of_finz_seq_between] ]%elem_of_list_fmap.
       solve_addr. }
     iFrame. iApply (IHl with "H H'"). solve_addr. solve_addr. }
-Qed.
+Qed. *)
 
-Lemma mbkregion_prepare `{memG Σ, cfgSG Σ} (a e : Addr) l l' :
-  (a + length l)%a = Some e →
-  (a + length l')%a = Some e →
+Lemma mbkregion_prepare `{memG Σ, cfgSG Σ} (a e : PhysAddr) l l' :
+  (a + length l)%pa = Some e →
+  (a + length l')%pa = Some e →
   ([∗ map] k↦v ∈ mkregion a e l, k ↦ₐ v) -∗
   ([∗ map] k↦v ∈ mkregion a e l', k ↣ₐ v) ==∗
   ([∗ map] k↦v ∈ mbkregion a e l l', k ↦ₐ v.1 ∗ k ↣ₐ v.2).
